\documentclass[preview]{standalone}
\usepackage{tikz,lmodern,amssymb}
\usepackage{knowledge}

\begin{document}

\begin{theo*}{Differentiability implies Continuity}
  If $f\left(x\right)$ is differentiable at $a$ then $f\left(x\right)$ is continuous at $a$ 
  \begin{pf}
    \begin{itemize}
     \item Because $f\left(x\right)$ is differentiable at $a$  we know that the following limit exists 
       \[
       f ^{ \prime }\left(a\right) = \lim_{x \to a } \frac{ f\left(x\right)  -  f\left(a\right)}{ x  -  a}
       \]
      \item We also note that the following limit exists as well:
        \[
        \lim_{x\to a} x  -  a = 0
        \]
      \item By the product law for limits we obtain that 
        \[
        \lim_{x \to a} \left[ \frac{f\left(x\right)  -  f\left(a\right)}{x  -  a}  \cdot  \left( x  -  a \right)  \right] = 0  \cdot  f ^{\prime}\left(a\right) = 0
        \]
        And note that  
        \[
          \lim_{x \to a} \left[ \frac{f\left(x\right)  -  f\left(a\right)}{x  -  a}  \cdot  \left( x  -  a \right)  \right] = \lim_{x \to a} \left[f\left(x\right)  -  f\left(a\right)  \right]
        \]
        \item Therefore
          \[
          \lim_{x \to a} \left[f\left(x\right)  -  f\left(a\right)  \right] = 0
          \]
        \item Since $\lim_{x \to a} f\left(a\right) = f\left(a\right)$ we can use the sum rule to obtain 
          \begin{align*}
            \lim_{x \to a} f\left(a\right)  +  \lim_{x \to a} \left[ f\left(x\right)  -  f\left(a\right) \right] &= \lim_{x \to a} \left[ f\left(a\right)  +  f\left(x\right)  -  f\left(a\right) \right] \\
                                                                                                                 &= \lim_{x \to a} f\left(x\right) 
          \end{align*}
        \item But recall that 
          \[
            \lim_{x \to a} f\left(a\right)  +  \lim_{x \to a} \left[ f\left(x\right)  -  f\left(a\right) \right]  = f\left(a\right)  +  0
          \]
        \item Thus we know that 
          \[
          \lim_{x \to a} f\left(x\right) = f\left(a\right)
          \]
          as required.
    \end{itemize}
  \end{pf}
\end{theo*}

\end{document}


